.

theories/FoL/InferenceRules.v
@@ -15,7 +15,7 @@ Import ListNotations.
 
 Context {L : language}.
 
-Definition varcouples : forall n, trms L n * trms L n :=
+Definition varcouples : forall n : nat, trms L n * trms L n :=
   nat_rec (fun n => (trms L n * trms L n)%type) (O_trms, O_trms) (fun n => prod_rec _ (fun lhs => fun rhs => (S_trms n (Var_trm (n + n)) lhs, S_trms n (Var_trm (S (n + n))) rhs))).
 
 Definition eqns_imp p : nat -> frm L :=
@@ -24,8 +24,8 @@ Definition eqns_imp p : nat -> frm L :=
 Definition Fun_eqAxm (f : L.(function_symbols)) : frm L :=
   eqns_imp (prod_rec (fun _ => frm L) (fun lhs => fun rhs => Eqn_frm (Fun_trm f lhs) (Fun_trm f rhs)) (varcouples (L.(function_arity_table) f))) (L.(function_arity_table) f).
 
-Definition Rel_eqAxm (r : L.(relation_symbols)) : frm L :=
-  eqns_imp (prod_rec (fun _ => frm L) (fun lhs => fun rhs => Imp_frm (Rel_frm r lhs) (Rel_frm r rhs)) (varcouples (L.(relation_arity_table) r))) (L.(relation_arity_table) r).
+Definition Rel_eqAxm (R : L.(relation_symbols)) : frm L :=
+  eqns_imp (prod_rec (fun _ => frm L) (fun lhs => fun rhs => Imp_frm (Rel_frm R lhs) (Rel_frm R rhs)) (varcouples (L.(relation_arity_table) R))) (L.(relation_arity_table) R).
 
 Inductive proof : list (frm L) -> frm L -> Set := (* Reference: "https://github.com/princeton-vl/CoqGym/blob/master/coq_projects/goedel/folProof.v#L68" *)
   | AXM p
@@ -35,8 +35,8 @@ Inductive proof : list (frm L) -> frm L -> Set := (* Reference: "https://github.
     (PF2 : proof ps2 p)
     : proof (ps1 ++ ps2) q
   | GEN ps q x
-    (NOT_FREE: forall p, In p ps -> is_not_free_in_frm x p)
-    (PF: proof ps q)
+    (NOT_FREE : forall p, In p ps -> is_not_free_in_frm x p)
+    (PF : proof ps q)
     : proof ps (All_frm x q)
   | IMP1 p q
     : proof [] (Imp_frm p (Imp_frm q p))
@@ -57,10 +57,10 @@ Inductive proof : list (frm L) -> frm L -> Set := (* Reference: "https://github.
     : proof [] (Imp_frm (Eqn_frm (Var_trm 0) (Var_trm 1)) (Eqn_frm (Var_trm 1) (Var_trm 0)))
   | EQN_TRANS
     : proof [] (Imp_frm (Eqn_frm (Var_trm 0) (Var_trm 1)) (Imp_frm (Eqn_frm (Var_trm 1) (Var_trm 2)) (Eqn_frm (Var_trm 0) (Var_trm 2))))
-  | EQN_FUNC f
+  | EQN_FUN f
     : proof [] (Fun_eqAxm f)
-  | EQN_REL r
-    : proof [] (Rel_eqAxm r).
+  | EQN_REL R
+    : proof [] (Rel_eqAxm R).
 
 Definition proves (Gamma : ensemble (frm L)) (C : frm L) : Prop :=
   exists ps, E.finite ps \subseteq Gamma /\ inhabited (proof ps C).
@@ -68,3 +68,90 @@ Definition proves (Gamma : ensemble (frm L)) (C : frm L) : Prop :=
 End HILBERT_PROOF_SYSTEM.
 
 End HPS.
+
+Module ND.
+
+Inductive infers {L : language} (Gamma : ensemble (frm L)) : forall C : frm L, Prop :=
+  | By_hyp p
+    (IN : p \in Gamma)
+    : Gamma ⊢ p
+  | Eqn_I t1
+    : Gamma ⊢ Eqn_frm t1 t1
+  | Eqn_E x t1 t2 p1
+    (INFERS1 : Gamma ⊢ Eqn_frm t1 t2)
+    (INFERS2 : Gamma ⊢ subst_frm (one_subst x t1) p1)
+    : Gamma ⊢ subst_frm (one_subst x t2) p1
+  | All_I x y p
+    (NOT_FREE1 : is_not_free_in_frms y Gamma)
+    (NOT_FREE2 : is_not_free_in_frm y (All_frm x p))
+    (INFERS1: Gamma ⊢ subst_frm (one_subst x (Var_trm y)) p)
+    : Gamma ⊢ All_frm x p
+  | All_E x t p
+    (INFERS1 : Gamma ⊢ All_frm x p)
+    : Gamma ⊢ subst_frm (one_subst x t) p
+  | Exs_I x t p
+    (INFERS1 : Gamma ⊢ subst_frm (one_subst x t) p)
+    : Gamma ⊢ Exs_frm x p
+  | Exs_E x y p1 p2
+    (NOT_FREE1 : is_not_free_in_frms y Gamma)
+    (NOT_FREE2 : is_not_free_in_frm y (Exs_frm x p1))
+    (NOT_FREE3 : is_not_free_in_frm y p2)
+    (INFERS1: Gamma ⊢ Exs_frm x p1)
+    (INFERS2: E.insert (subst_frm (one_subst x (Var_trm y)) p1) Gamma ⊢ p2)
+    : Gamma ⊢ p2
+  | Bot_I p1
+    (INFERS1 : Gamma ⊢ p1)
+    (INFERS2 : Gamma ⊢ Neg_frm p1)
+    : Gamma ⊢ Bot_frm
+  | Bot_E p1
+    (INFERS1 : Gamma ⊢ Bot_frm)
+    : Gamma ⊢ p1
+  | Neg_I p1
+    (INFERS1: E.insert p1 Gamma ⊢ Bot_frm)
+    : Gamma ⊢ Neg_frm p1
+  | Neg_E p1
+    (INFERS1 : E.insert (Neg_frm p1) Gamma ⊢ Bot_frm)
+    : Gamma ⊢ p1
+  | Con_I p1 p2
+    (INFERS1 : Gamma ⊢ p1)
+    (INFERS2 : Gamma ⊢ p2)
+    : Gamma ⊢ Con_frm p1 p2
+  | Con_E1 p1 p2
+    (INFERS1 : Gamma ⊢ Con_frm p1 p2)
+    : Gamma ⊢ p1
+  | Con_E2 p1 p2
+    (INFERS1 : Gamma ⊢ Con_frm p1 p2)
+    : Gamma ⊢ p2
+  | Dis_I1 p1 p2
+    (INFERS1 : Gamma ⊢ p1)
+    : Gamma ⊢ Dis_frm p1 p2
+  | Dis_I2 p1 p2
+    (INFERS1 : Gamma ⊢ p2)
+    : Gamma ⊢ Dis_frm p1 p2
+  | Dis_E p1 p2 p3
+    (INFERS1 : Gamma ⊢ Dis_frm p1 p2)
+    (INFERS2 : E.insert p1 Gamma ⊢ p3)
+    (INFERS3 : E.insert p2 Gamma ⊢ p3)
+    : Gamma ⊢ p3
+  | Imp_I p1 p2
+    (INFERS1 : E.insert p1 Gamma ⊢ p2)
+    : Gamma ⊢ Imp_frm p1 p2
+  | Imp_E p1 p2
+    (INFERS1 : Gamma ⊢ Imp_frm p1 p2)
+    (INFERS2 : Gamma ⊢ p1)
+    : Gamma ⊢ p2
+  | Iff_I p1 p2
+    (INFERS1 : E.insert p1 Gamma ⊢ p2)
+    (INFERS2 : E.insert p2 Gamma ⊢ p1)
+    : Gamma ⊢ Iff_frm p1 p2
+  | Iff_E1 p1 p2
+    (INFERS1 : Gamma ⊢ Iff_frm p1 p2)
+    (INFERS2 : Gamma ⊢ p1)
+    : Gamma ⊢ p2
+  | Iff_E2 p1 p2
+    (INFERS1 : Gamma ⊢ Iff_frm p1 p2)
+    (INFERS2 : Gamma ⊢ p2)
+    : Gamma ⊢ p1
+  where " Gamma ⊢ C " := (infers Gamma C) : type_scope.
+
+End ND.
