theories/FoL/MetaTh.v
@@ -1,0 +1,11 @@
+Require Import LoL.Prelude.Prelude.
+Require Import LoL.Prelude.LEM.
+Require Import LoL.Prelude.Notations.
+Require Import LoL.Math.ThN.
+Require Import LoL.Data.Vector.
+Require Import LoL.FoL.Syntax.
+Require Import LoL.FoL.Semantics.
+Require Import LoL.FoL.InferenceRules.
+
+#[local] Infix "\in" := E.elem.
+#[local] Infix "\subseteq" := E.isSubsetOf.
